Geometry/Theory.lean
@@ -3,7 +3,7 @@
 import Geometry.Theory.Set
 import Geometry.Theory.Distinct
 import Geometry.Theory.Forgetting
-import Geometry.Theory.Arranged
+import Geometry.Theory.Extending
 
 import Geometry.Theory.Axioms
 import Geometry.Theory.Ch1
